Qed wpc for server's `main()`

src/program_proof/ctrexample/interface.v
@@ -20,10 +20,10 @@ Context `{HPRE: !gooseGlobalGS Σ}.
 (* HOCAP-style spec *)
 Program Definition FAISpec (γ:gname) : savedSpecO Σ (list u8) (list u8) :=
   λ reqData, λne (Φ : list u8 -d> iPropO Σ),
-  (□(
+  (
       ∀ (x:nat), counter_own γ x ={⊤}=∗ counter_own γ (x + 1) ∗
                                     (∀ l, ⌜has_encoding l [EncUInt64 x]⌝ -∗ Φ l)
-    ))%I
+    )%I
 .
 Next Obligation.
   solve_proper.
@@ -32,11 +32,11 @@ Defined.
 (* TaDa-style spec *)
 Program Definition FAISpec_tada (γ:gname) : savedSpecO Σ (list u8) (list u8) :=
   λ reqData, λne (Φ : list u8 -d> iPropO Σ),
-  (□(
+  (
        ∃ Eo Ei,
        |={Eo,Ei}=> ∃ x, counter_own γ x ∗
                       (counter_own γ (x+1) ={Ei,Eo}=∗ (∀ l, ⌜has_encoding l [EncUInt64 x]⌝ -∗ Φ l))
-    ))%I
+    )%I
 .
 
 Next Obligation.
